supporting zext

coq/DynamicValue.v
@@ -196,59 +196,12 @@ Definition eval_icmp (op : icmp) (v1 v2 : dynamic_value) : option dynamic_value 
 (* TODO: handle i16 *)
 Definition convert conv x t1 t2 : option dynamic_value :=
   match conv with
-  | Trunc =>
-    match t1, x, t2 with
-    | TYPE_I 8, DV_Int (DI_I8 i1), TYPE_I 1 =>
-      Some (DV_Int (DI_I1 (repr (unsigned i1))))
-    | TYPE_I 32, DV_Int (DI_I32 i1), TYPE_I 1 =>
-      Some (DV_Int (DI_I1 (repr (unsigned i1))))
-    | TYPE_I 32, DV_Int (DI_I32 i1), TYPE_I 8 =>
-      Some (DV_Int (DI_I8 (repr (unsigned i1))))
-    | TYPE_I 64, DV_Int (DI_I64 i1), TYPE_I 1 =>
-      Some (DV_Int (DI_I1 (repr (unsigned i1))))
-    | TYPE_I 64, DV_Int (DI_I64 i1), TYPE_I 8 =>
-      Some (DV_Int (DI_I8 (repr (unsigned i1))))
-    | TYPE_I 64, DV_Int (DI_I64 i1), TYPE_I 32 =>
-      Some (DV_Int (DI_I32 (repr (unsigned i1))))
-    | _, _, _ => None
-    end
   | Zext =>
     match t1, x, t2 with
-    | TYPE_I 1, DV_Int (DI_I1 i1), TYPE_I 8 =>
-      Some (DV_Int (DI_I8 (repr (unsigned i1))))
-    | TYPE_I 1, DV_Int (DI_I1 i1), TYPE_I 32 =>
-      Some (DV_Int (DI_I32 (repr (unsigned i1))))
-    | TYPE_I 1, DV_Int (DI_I1 i1), TYPE_I 64 =>
-      Some (DV_Int (DI_I64 (repr (unsigned i1))))
-    | TYPE_I 8, DV_Int (DI_I8 i1), TYPE_I 32 =>
-      Some (DV_Int (DI_I32 (repr (unsigned i1))))
-    | TYPE_I 8, DV_Int (DI_I8 i1), TYPE_I 64 =>
-      Some (DV_Int (DI_I64 (repr (unsigned i1))))
     | TYPE_I 32, DV_Int (DI_I32 i1), TYPE_I 64 =>
       Some (DV_Int (DI_I64 (repr (unsigned i1))))
     | _, _, _ => None
     end
-  | Sext =>
-    match t1, x, t2 with
-    | TYPE_I 1, DV_Int (DI_I1 i1), TYPE_I 8 =>
-      Some (DV_Int (DI_I8 (repr (signed i1))))
-    | TYPE_I 1, DV_Int (DI_I1 i1), TYPE_I 32 =>
-      Some (DV_Int (DI_I32 (repr (signed i1))))
-    | TYPE_I 1, DV_Int (DI_I1 i1), TYPE_I 64 =>
-      Some (DV_Int (DI_I64 (repr (signed i1))))
-    | TYPE_I 8, DV_Int (DI_I8 i1), TYPE_I 32 =>
-      Some (DV_Int (DI_I32 (repr (signed i1))))
-    | TYPE_I 8, DV_Int (DI_I8 i1), TYPE_I 64 =>
-      Some (DV_Int (DI_I64 (repr (signed i1))))
-    | TYPE_I 32, DV_Int (DI_I32 i1), TYPE_I 64 =>
-      Some (DV_Int (DI_I64 (repr (signed i1))))
-    | _, _, _ => None
-    end
-  | Bitcast =>
-    match t1, x, t2 with
-    | TYPE_I bits1, x, TYPE_I bits2 =>
-      if (bits1 =? bits2)%positive then Some x else None
-    | _, _, _ => None
-    end
+  | _ => None
   end
 .
