coq/Completeness.v
@@ -260,6 +260,38 @@ Proof.
       apply OA_None.
     }
   }
+  {
+    apply IHe with (ot := (Some t1)) in H4.
+    destruct (eval_exp c_ls c_gs (Some t1) e) as [dv | ] eqn:E.
+    {
+      inversion H1; subst.
+      inversion H4; subst.
+      destruct t1; try apply OA_None.
+      destruct t2;
+      try (
+        simpl;
+        repeat (destruct w; try apply OA_None);
+        destruct (make_dynamic_int sort (smt_eval_ast m sort ast)); apply OA_None
+      ).
+      {
+        rename w into w1, w0 into w2.
+        repeat (destruct w1; try apply OA_None).
+        {
+          simpl.
+          destruct sort; try apply OA_None.
+          repeat (destruct w2; try apply OA_None).
+          simpl.
+          eapply OA_Some.
+          { reflexivity. }
+          { simpl. reflexivity. }
+        }
+      }
+    }
+    {
+      inversion H4; subst.
+      apply OA_None.
+    }
+  }
 Qed.
 
 Lemma empty_store_correspondence : forall m,
